code/nist-pcurves/Hacl.Impl.PCurves.PointMul.fsti
@@ -17,14 +17,13 @@ open Hacl.Impl.PCurves.Point
 module S = Spec.PCurves
 
 include Hacl.Impl.PCurves.Group
-include Hacl.PCurves.PrecompTable
+include Hacl.Impl.PCurves.PrecompTable
 
 
 #set-options "--z3rlimit 30 --fuel 0 --ifuel 0"
-[@(strict_on_arguments [0;1;2;3;4;5;6])]
 noextract inline_for_extraction
-val point_mul {| cp:S.curve_params |} {| curve_constants |} {| bn_ops |} {| f:field_ops |}
-              {| curve_inv_sqrt|} {| point_ops |} {| pt:precomp_tables |}:
+let point_mul_t {| cp:S.curve_params |} {| curve_constants |} {| bn_ops |} {| f:field_ops |}
+              {| curve_inv_sqrt|} {| point_ops |} {| pt:precomp_tables |} =
   res:point -> scalar:felem -> p:point -> Stack unit
   (requires fun h ->
     live h p /\ live h res /\ live h scalar /\
@@ -35,11 +34,15 @@ val point_mul {| cp:S.curve_params |} {| curve_constants |} {| bn_ops |} {| f:fi
     S.to_aff_point (from_mont_point (as_point_nat h1 res)) ==
     S.to_aff_point (S.point_mul (as_nat h0 scalar) (from_mont_point (as_point_nat h0 p))))
 
-
 [@(strict_on_arguments [0;1;2;3;4;5;6])]
 noextract inline_for_extraction
-val point_mul_g {| cp:S.curve_params |} {| curve_constants |} {| bn_ops |} {| f:field_ops |}
-                {| curve_inv_sqrt|} {| point_ops |} {| pt:precomp_tables |}:
+val point_mul_gen {| cp:S.curve_params |} {| curve_constants |} {| bn_ops |} {| f:field_ops |}
+              {| curve_inv_sqrt|} {| point_ops |} {| pt:precomp_tables |}: point_mul_t
+
+
+noextract inline_for_extraction
+let point_mul_g_t {| cp:S.curve_params |} {| curve_constants |} {| bn_ops |} {| f:field_ops |}
+                {| curve_inv_sqrt|} {| point_ops |} {| pt:precomp_tables |} =
   res:point -> scalar:felem -> Stack unit
   (requires fun h ->
     live h res /\ live h scalar /\ disjoint res scalar /\
@@ -49,11 +52,14 @@ val point_mul_g {| cp:S.curve_params |} {| curve_constants |} {| bn_ops |} {| f:
     S.to_aff_point (from_mont_point (as_point_nat h1 res)) ==
     S.to_aff_point (S.point_mul_g (as_nat h0 scalar)))
 
-
 [@(strict_on_arguments [0;1;2;3;4;5;6])]
 noextract inline_for_extraction
-val point_mul_double_g {| cp:S.curve_params |} {| curve_constants |} {| bn_ops |} {| f:field_ops |}
-                       {| curve_inv_sqrt|} {| point_ops |} {| pt:precomp_tables |}:
+val point_mul_g_gen {| cp:S.curve_params |} {| curve_constants |} {| bn_ops |} {| f:field_ops |}
+                {| curve_inv_sqrt|} {| point_ops |} {| pt:precomp_tables |}: point_mul_g_t
+
+noextract inline_for_extraction
+let point_mul_double_g_t {| cp:S.curve_params |} {| curve_constants |} {| bn_ops |} {| f:field_ops |}
+                       {| curve_inv_sqrt|} {| point_ops |} {| pt:precomp_tables |} = 
   res:point -> scalar1:felem -> scalar2:felem -> p:point -> Stack unit
   (requires fun h ->
     live h res /\ live h scalar1 /\ live h scalar2 /\ live h p /\
@@ -65,3 +71,17 @@ val point_mul_double_g {| cp:S.curve_params |} {| curve_constants |} {| bn_ops |
     S.to_aff_point (from_mont_point (as_point_nat h1 res)) ==
     S.to_aff_point (S.point_mul_double_g (as_nat h0 scalar1) (as_nat h0 scalar2)
       (from_mont_point (as_point_nat h0 p))))
+
+[@(strict_on_arguments [0;1;2;3;4;5;6])]
+noextract inline_for_extraction
+val point_mul_double_g_gen {| cp:S.curve_params |} {| curve_constants |} {| bn_ops |} {| f:field_ops |}
+                       {| curve_inv_sqrt|} {| point_ops |} {| pt:precomp_tables |}: point_mul_double_g_t
+
+
+inline_for_extraction
+class point_mul_ops {| cp:S.curve_params |} {| curve_constants |} {| bn_ops |} {| f:field_ops |}
+                    {| curve_inv_sqrt|} {| point_ops |} {| pt:precomp_tables |} = {
+      point_mul: point_mul_t;
+      point_mul_g: point_mul_g_t;
+      point_mul_double_g: point_mul_double_g_t
+}
