code/nist-pcurves/Hacl.Impl.PCurves.PointMul.P256.fst
@@ -1,0 +1,53 @@
+module Hacl.Impl.PCurves.PointMul.P256
+
+open FStar.HyperStack
+open FStar.HyperStack.ST
+open FStar.Mul
+
+open Lib.IntTypes
+open Lib.Buffer
+
+module ST = FStar.HyperStack.ST
+module LSeq = Lib.Sequence
+
+module BE = Hacl.Impl.Exponentiation.Definitions
+
+module S = Spec.PCurves
+module SL = Spec.PCurves.Lemmas
+
+open Hacl.Impl.PCurves.Bignum
+open Hacl.Impl.PCurves.Field
+open Hacl.Impl.PCurves.Constants
+open Hacl.Impl.PCurves.InvSqrt
+open Hacl.Impl.PCurves.Point
+
+open Spec.P256
+open Hacl.Impl.PCurves.Constants.P256
+open Hacl.Impl.PCurves.Bignum.P256
+open Hacl.Impl.PCurves.Field.P256
+open Hacl.Impl.PCurves.Finv.P256
+open Hacl.Impl.PCurves.Qinv.P256
+open Hacl.Impl.PCurves.Group.P256
+open Hacl.Impl.PCurves.PrecompTable.P256
+open Hacl.Impl.PCurves.PointMul
+
+[@CInline]
+val point_mul: point_mul_t
+let point_mul = point_mul_gen
+
+[@CInline]
+val point_mul_g: point_mul_g_t
+let point_mul_g = point_mul_g_gen
+
+[@CInline]
+val point_mul_double_g: point_mul_double_g_t
+let point_mul_double_g = point_mul_double_g_gen
+
+inline_for_extraction
+instance p256_point_mul_ops : point_mul_ops = {
+  point_mul;
+  point_mul_g;
+  point_mul_double_g
+}
+
+
